A Linear Diophantine Equation (in two variables) is an equation of the general form:
$$ax+by=c$$
where $a, b, c$ are given integers and $x, y$ are unknown integers.
### Degenerate Case
A degenerate case is when $a=b=0$. Either we have no solutions or infinitely many solutions, depending on whether $c=0$ or not.
### Analytic Solution
When $a\ne 0$ and $b\ne 0$, the equation can be equivalently treated as either of the following:
$$
\begin{align}
ax\equiv c\pmod b\\
by\equiv c\pmod a
\end{align}
$$
Without loss of generality, assume that $b\ne 0$ and consider the first equation. When $a$ and $b$ are co-prime, the solution to it is given as:
$$x\equiv ca^{-1}\pmod b$$
where $a^{-1}$ is the [[Modular Arithmetic#Modular Inverse|Modular Inverse]] of $a$ modulo $b$.
When $a$ and $b$ are not co-prime, values of $ax$ modulo $b$ for all integer $x$ are divisible by $g=gcd(a, b)$, so the solution only exists when $c$ is divisible by $g$. In such a case, one of the solutions can be found by reducing the equation by $g$:
$$\left(\frac{a}{g}\right)x\equiv \left(\frac{c}{g}\right) \pmod{b/g}$$
By the definition of $g$, the numbers $\frac{a}{g}$ and $\frac{b}{g}$ are co-prime, so the solution is given explicitly as:
$$
\begin{align}
x &\equiv \left(\frac{c}{g}\right)\left(\frac{a}{g}\right)^{-1}\pmod{b/g}\\
y &= \frac{c-ax}{b}
\end{align}
$$
### Algorithmic Solution
To find one solution of the Diophantine Equation with 2 unknowns, we use the [[Euclidean Algorithm#Extended Euclidean Algorithm|Extended Euclidean Algorithm]].
First, assume that $a$ and $b$ are non-negative:
$$ax_g+by_g=g$$
If $c$ is divisible by $g=\gcd(a, b)$, then the diophantine equation has a solution, otherwise it does not have any solution.
Assuming $c$ is divisible by $g$:
$$ax_g\cdot\frac{c}{g}+by_g\cdot\frac{c}{g} = c$$
Therefore, **one of the solutions** of the diophantine equation is:
$$
\begin{align}
x_0 &= x_g\cdot{c}{g}\\
y_0 &= y_g\cdot{c}{g}
\end{align}
$$
```cpp
int gcdExtendedRecursive(int a, int b, int& x, int& y)
{
	if (b == 0)
	{
		x = 1;
		y = 0;
		return a;
	}
	int x1, y1;
	int d = gcd(b, a % b, x1, y1);
	x = y1;
	y = x1 - y1*(a/b);
	return d;
}

bool findAnySolution(int a, int b, int c, int& x0, int& y0, int& g)
{
	g = gcdExtendedRecursive(abs(a), abs(b), x0, y0);
	if (c % g)
		return false;
	x0 *= c / g;
	y0 *= c / g;
	// handle negative inputs
	if (a < 0)
		x0 = -x0;
	if (b < 0)
		y0 = -y0;
	return true;
}
```
#### Getting All Solutions
We now have $x_0, y_0$ which satisfy he following:
$$ax_0+by_0=c$$
We can see that adding $k\cdot \frac{b}{g}$ to $x_0$ while subtracting $k\cdot\frac{a}{g}$ from $y_0$ does not break the equality:
$$
a\left(x_0+k\frac{b}{g}\right)+b\left(y_0-k\frac{a}{g}\right)
= ax_0+by_0 = c
$$
From this, we can find all the solutions of the diophantine equation, which are of the form:
$$
\begin{align}
x &= x_0+k\frac{b}{g}\\
y &= y_0-k\frac{a}{g}
\end{align}
$$